\documentclass{article}
\usepackage{amsmath}

\newcommand{\wrap}[1]{\left( #1 \right)}

\title{Notes on Fast Fourier Transforms}
\author{Samuel}
\begin{document}

Given $(x_0,\cdots,x_{2^N})$, we wish to find:
$$\tilde{x}_k = \sum_{j=0}^{2^N-1}
                  \exp\wrap{-i \frac{\tau k}{2^N} j} x_j$$
Notice that we can decompose:
\begin{align}
  \tilde{x}_k &= \sum_{j=0}^{2^{N-1}-1}
                   \exp\wrap{-i \frac{\tau \boxed{2}k}{\boxed{2^N}} j}
                   \wrap{x_{2j} + \exp\wrap{-i \frac{\tau k}{2^N}} x_{2j+1}} \\
              &= \tilde{y}_k + \exp\wrap{-i \frac{\tau k}{2^N}} \tilde{z}_k
\end{align}
Here, $y_j=x_{2j}$ and $z_j=x_{2j+1}$ are alternating subsequences of our original inputs.
The second equality follows when we notice the $\boxed{\text{boxed}}$ $2$'s cancel.
Also note that there are only $2^{N-1}$ total $\tilde{y}$'s; after that they wrap around.
Same with $\tilde{z}$'s.
\end{document}
